examples/primitives/Crypto.HMAC.Sha512.fst
@@ -8,60 +8,66 @@ open Crypto.Sha512
 
 
 
-(* Define a function to wrap the key length after 128 bits *)
+(* Define parameters *)
+let hash = sha512
+let hl = 64
+let bl = 128
+
+(* Define a function to wrap the key length after bl bits *)
 val wrap_key : (key    :sbytes) ->
                (keylen :nat { length key = keylen })
-               -> St (okey:sbytes { length okey <= 128 } * okeylen: nat)
+               -> St (okey:sbytes { length okey <= bl } * okeylen: nat)
 
 let wrap_key key keylen =
-  if keylen > 128 then
-    let nkey = create #8 FStar.UInt8.zero 32 in
-    sha512 nkey key keylen;
-    nkey,32
+  if keylen > bl then
+    let nkey = create #8 FStar.UInt8.zero hl in
+    hash nkey key keylen;
+    nkey,hl
   else
     key,keylen
 
+
 (* Define the main function *)
-val hmac_sha512: (mac     :sbytes { length mac = 32 }) ->
-                 (key     :sbytes { Disjoint key mac }) ->
-                 (keylen  :nat { length key = keylen }) ->
-                 (data    :sbytes { Disjoint mac data /\ Disjoint key data }) ->
-                 (datalen :nat { length data = datalen })
-                 -> ST unit
+val hmac_sha512 : (mac     :sbytes { length mac = hl }) ->
+                  (key     :sbytes { Disjoint key mac }) ->
+                  (keylen  :nat      { length key = keylen }) ->
+                  (data    :sbytes { Disjoint mac data /\ Disjoint key data }) ->
+                  (datalen :nat      { length data = datalen })
+                  -> ST unit
                       (requires (fun h -> Live h mac /\ Live h data /\ Live h key))
                       (ensures  (fun h0 r h1 -> Live h1 mac /\ Live h1 data /\ Live h1 key))
 
 let hmac_sha512 mac key keylen data datalen =
   (* Define ipad and opad *)
-  let ipad = SBuffer.create #8 (FStar.UInt8.of_string "0x36") 128 in
-  let opad = SBuffer.create #8 (FStar.UInt8.of_string "0x5c") 128 in
+  let ipad = SBuffer.create #8 (FStar.UInt8.of_string "0x36") bl in
+  let opad = SBuffer.create #8 (FStar.UInt8.of_string "0x5c") bl in
 
   (* Step 1: make sure the key has the proper length *)
   let okey,okeylen = wrap_key key keylen in
-  let s1 = create #8 FStar.UInt8.zero 128 in
+  let s1 = create #8 FStar.UInt8.zero bl in
   FStar.SBytes.blit okey 0 s1 0 okeylen;
 
   (* Step 2: xor "result of step 1" with ipad *)
-  let s2 = create #8 FStar.UInt8.zero 128 in
-  FStar.SBytes.xor_bytes s2 s1 ipad 128;
+  let s2 = create #8 FStar.UInt8.zero bl in
+  FStar.SBytes.xor_bytes s2 s1 ipad bl;
 
   (* Step 3: append data to "result of step 2" *)
-  let s3 = create #8 FStar.UInt8.zero (128 + datalen) in
-  FStar.SBytes.blit s2 0 s3 0 128;
-  FStar.SBytes.blit data 0 s3 128 datalen;
+  let s3 = create #8 FStar.UInt8.zero (bl + datalen) in
+  FStar.SBytes.blit s2 0 s3 0 bl;
+  FStar.SBytes.blit data 0 s3 bl datalen;
 
   (* Step 4: apply H to "result of step 3" *)
-  let s4 = create #8 FStar.UInt8.zero 32 in
-  sha512 s4 s3 (128 + datalen);
+  let s4 = create #8 FStar.UInt8.zero hl in
+  hash s4 s3 (bl + datalen);
 
   (* Step 5: xor "result of step 1" with opad *)
-  let s5 = create #8 FStar.UInt8.zero 128 in
-  FStar.SBytes.xor_bytes s5 s1 opad 128;
+  let s5 = create #8 FStar.UInt8.zero bl in
+  FStar.SBytes.xor_bytes s5 s1 opad bl;
 
   (* Step 6: append "result of step 4" to "result of step 5" *)
-  let s6 = create #8 FStar.UInt8.zero (32 + 128) in
-  FStar.SBytes.blit s5 0 s6 0 128;
-  FStar.SBytes.blit s4 0 s6 128 32;
+  let s6 = create #8 FStar.UInt8.zero (hl + bl) in
+  FStar.SBytes.blit s5 0 s6 0 bl;
+  FStar.SBytes.blit s4 0 s6 bl hl;
 
   (* Step 7: apply H to "result of step 6" *)
-  sha512 mac s6 (32 + 128)
+  hash mac s6 (hl + bl)
